

# MA265 Methods of Mathematical Modelling 3, Assignment 3

Dyson Dyson

## Question 1

*Fourier series:* For integers  $m$  and  $n$ , show that

$$\begin{aligned}\int_{-\pi}^{\pi} \sin(mx) \sin(nx) \, dx &= \begin{cases} \pi & \text{if } m = n \\ 0 & \text{otherwise,} \end{cases} \\ \int_{-\pi}^{\pi} \cos(mx) \cos(nx) \, dx &= \begin{cases} \pi & \text{if } m = n \\ 0 & \text{otherwise,} \end{cases}\end{aligned}$$

and

$$\int_{-\pi}^{\pi} \sin(mx) \cos(nx) \, dx = 0 \quad \text{for all } m \text{ and } n.$$

Consider the function  $\phi(x) = x$  on  $[-\pi, \pi]$ . Assuming  $\phi$  can be written in the form

$$\phi(x) = a_0 + \sum_{k=1}^{\infty} a_k \cos(kx) + b_k \sin(kx), \quad (1)$$

find the values of the coefficients  $a_k$  and  $b_k$ .

We will first consider the integral of  $\sin(mx) \sin(nx)$ . If  $m = n$ , the integral becomes

$$\begin{aligned}\int_{-\pi}^{\pi} \sin(mx) \sin(nx) \, dx &= \int_{-\pi}^{\pi} \sin^2(nx) \, dx \\ &= \frac{1}{2} \int_{-\pi}^{\pi} (1 - \cos(2nx)) \, dx \\ &= \frac{1}{2} \left[ x - \frac{1}{2n} \sin(2nx) \right]_{-\pi}^{\pi} \\ &= \frac{1}{2} \left( \pi - \frac{1}{2n} \sin(2n\pi) - \left( -\pi - \frac{1}{2n} \sin(-2n\pi) \right) \right) \\ &= \frac{1}{2} \left( \pi - \frac{1}{2n} \sin(2n\pi) + \pi + \frac{1}{2n} \sin(-2n\pi) \right)\end{aligned}$$

$$\begin{aligned}
&= \frac{1}{2} \left( 2\pi - \frac{1}{2n} \sin(2n\pi) - \frac{1}{2n} \sin(2n\pi) \right) \\
&= \pi.
\end{aligned}$$

If instead  $m \neq n$ , we get

$$\begin{aligned}
\int_{-\pi}^{\pi} \sin(mx) \sin(nx) \, dx &= \int_{-\pi}^{\pi} \frac{-\cos(mx + nx) + \cos(mx - nx)}{2} \, dx \\
&= \frac{1}{2} \left[ \frac{-1}{m+n} \sin(mx + nx) + \frac{1}{m-n} \sin(mx - nx) \right]_{-\pi}^{\pi} \\
&= \frac{1}{2} \left( \frac{-1}{m+n} \sin((m+n)\pi) + \frac{1}{m-n} \sin((m-n)\pi) \right. \\
&\quad \left. + \frac{1}{m+n} \sin(-(m+n)\pi) - \frac{1}{m-n} \sin(-(m-n)\pi) \right) \\
&= 0
\end{aligned}$$

since  $m+n$  and  $m-n$  are always integers, so  $\sin((m+n)\pi)$  etc. are all 0.

We will now consider the integral of  $\cos(mx) \cos(nx)$ . As before, if  $m = n$ , the integral becomes

$$\begin{aligned}
\int_{-\pi}^{\pi} \cos(mx) \cos(nx) \, dx &= \int_{-\pi}^{\pi} \cos^2(nx) \, dx \\
&= \frac{1}{2} \int_{-\pi}^{\pi} (1 + \cos(2nx)) \, dx \\
&= \frac{1}{2} \left[ x + \frac{1}{2n} \sin(2nx) \right]_{-\pi}^{\pi} \\
&= \frac{1}{2} \left( \pi + \frac{1}{2n} \sin(2n\pi) - \left( -\pi + \frac{1}{2n} \sin(-2n\pi) \right) \right) \\
&= \frac{1}{2} \left( \pi + \frac{1}{2n} \sin(2n\pi) + \pi - \frac{1}{2n} \sin(-2n\pi) \right) \\
&= \frac{1}{2} \left( 2\pi + \frac{1}{2n} \sin(2n\pi) + \frac{1}{2n} \sin(2n\pi) \right) \\
&= \pi + \frac{1}{2n} \sin(2n\pi) \\
&= \pi
\end{aligned}$$

since  $n \in \mathbb{Z}$ , so  $\sin(2n\pi)$  is always 0.

If instead  $m \neq n$ , we get

$$\begin{aligned}
 \int_{-\pi}^{\pi} \cos(mx) \cos(nx) \, dx &= \int_{-\pi}^{\pi} \frac{\cos(mx + nx) + \cos(mx - nx)}{2} \, dx \\
 &= \frac{1}{2} \left[ \frac{1}{m+n} \sin(mx + nx) + \frac{1}{m-n} \sin(mx - nx) \right]_{-\pi}^{\pi} \\
 &= \frac{1}{2} \left( \frac{1}{m+n} \sin((m+n)\pi) + \frac{1}{m-n} \sin((m-n)\pi) \right. \\
 &\quad \left. - \frac{1}{m+n} \sin(-(m+n)\pi) - \frac{1}{m-n} \sin(-(m-n)\pi) \right) \\
 &= 0
 \end{aligned}$$

since  $m+n$  and  $m-n$  are always integers, so  $\sin((m+n)\pi)$  etc. are all 0.

We will now consider the integral of  $\sin(mx) \cos(nx)$ . For any  $m$  and  $n$ ,

$$\begin{aligned}
 \int_{-\pi}^{\pi} \sin(mx) \cos(nx) \, dx &= \int_{-\pi}^{\pi} \frac{\sin(mx + nx) + \sin(mx - nx)}{2} \, dx \\
 &= \frac{1}{2} \left[ \frac{-1}{m+n} \cos(mx + nx) - \frac{1}{m-n} \cos(mx - nx) \right]_{-\pi}^{\pi} \\
 &= \frac{1}{2} \left( \frac{-1}{m+n} \cos((m+n)\pi) - \frac{1}{m-n} \cos((m-n)\pi) \right. \\
 &\quad \left. + \frac{1}{m+n} \cos(-(m+n)\pi) + \frac{1}{m-n} \cos(-(m-n)\pi) \right) \\
 &= \frac{1}{2} \left( \frac{-1}{m+n} \cos((m+n)\pi) - \frac{1}{m-n} \cos((m-n)\pi) \right. \\
 &\quad \left. + \frac{1}{m+n} \cos((m+n)\pi) + \frac{1}{m-n} \cos((m-n)\pi) \right) \\
 &= 0.
 \end{aligned}$$

To find  $a_k$  in the Fourier series for  $\phi$ , we can multiply both sides by  $\cos(nx)$  and integrate. On the LHS, we get

$$\begin{aligned}
 \int_{-\pi}^{\pi} x \cos(nx) \, dx &= \left[ \frac{nx \sin(nx) + \cos(nx)}{n^2} \right]_{-\pi}^{\pi} \\
 &= \frac{n\pi \sin(n\pi) + \cos(n\pi) - (-n\pi \sin(-n\pi) + \cos(-n\pi))}{n^2} \\
 &= \frac{n\pi \sin(n\pi) + n\pi \sin(-n\pi) + \cos(n\pi) - \cos(-n\pi)}{n^2} \\
 &= \frac{n\pi \sin(n\pi) - n\pi \sin(n\pi) + \cos(n\pi) - \cos(n\pi)}{n^2} \\
 &= 0.
 \end{aligned}$$

On the RHS, we get

$$\begin{aligned}
 & a_0 \cos(nx) + \sum_{k=1}^{\infty} a_k \cos(kx) \cos(nx) + b_k \sin(kx) \cos(nx) \\
 &= \int_{-\pi}^{\pi} \left( a_0 \cos(nx) + \sum_{k=1}^{\infty} a_k \cos(kx) \cos(nx) + b_k \sin(kx) \cos(nx) \right) dx \\
 &= a_0 \int_{-\pi}^{\pi} \cos(nx) dx + \sum_{k=1}^{\infty} \left( a_k \int_{-\pi}^{\pi} \cos(kx) \cos(nx) dx \right. \\
 &\quad \left. + b_k \int_{-\pi}^{\pi} \sin(kx) \cos(nx) dx \right) \\
 &= 0 + \sum_{k=1}^{\infty} a_k \int_{-\pi}^{\pi} \cos(kx) \cos(nx) dx \\
 &= 0a_0 + 0a_1 + \cdots + 0a_{n-1} + \pi a_n + 0a_{n+1} \cdots \\
 &= \pi a_n.
 \end{aligned}$$

So  $a_n = 0$ .

We can do the same to find  $b_k$ , but with  $\sin(nx)$ . On the LHS, we get

$$\begin{aligned}
 \int_{-\pi}^{\pi} x \sin(nx) dx &= \left[ \frac{\sin(nx) - nx \cos(nx)}{n^2} \right]_{-\pi}^{\pi} \\
 &= \frac{\sin(n\pi) - n\pi \cos(n\pi) - (\sin(-n\pi) - n(-\pi) \cos(-n\pi))}{n^2} \\
 &= \frac{\sin(n\pi) - \sin(-n\pi) - n\pi \cos(n\pi) - n\pi \cos(-n\pi)}{n^2} \\
 &= \frac{\sin(n\pi) + \sin(n\pi) - n\pi \cos(n\pi) - n\pi \cos(n\pi)}{n^2} \\
 &= \frac{2 \sin(n\pi) - 2n\pi \cos(n\pi)}{n^2}.
 \end{aligned}$$

On the RHS, we get

$$\begin{aligned}
 & a_0 \sin(nx) + \sum_{k=1}^{\infty} a_k \cos(kx) \sin(nx) + b_k \sin(kx) \sin(nx) \\
 &= \int_{-\pi}^{\pi} \left( a_0 \sin(nx) + \sum_{k=1}^{\infty} a_k \cos(kx) \sin(nx) + b_k \sin(kx) \sin(nx) \right) dx \\
 &= a_0 \int_{-\pi}^{\pi} \sin(nx) dx + \sum_{k=1}^{\infty} \left( a_k \int_{-\pi}^{\pi} \cos(kx) \sin(nx) dx \right. \\
 &\quad \left. + b_k \int_{-\pi}^{\pi} \sin(kx) \sin(nx) dx \right) \\
 &= 0 + \sum_{k=1}^{\infty} b_k \int_{-\pi}^{\pi} \sin(kx) \sin(nx) dx \\
 &= 0b_0 + 0b_1 + \cdots + 0b_{n-1} + \pi b_n + 0b_{n+1} \cdots \\
 &= \pi b_n.
 \end{aligned}$$

So  $b_n = \frac{2 \sin(n\pi) - 2n\pi \cos(n\pi)}{n^2 \pi}.$

## Question 2

*Fourier series:* Let  $\phi : [-\pi, \pi] \rightarrow \mathbb{R}$  be an even function. Prove that  $\hat{\phi}(k) = \hat{\phi}(-k)$ . Further, show that the Fourier series of  $\phi$  is a cosine series, in the sense that

$$S_n[\phi](x) = \hat{\phi}(0) + 2 \sum_{k=1}^n \hat{\phi}(k) \cos(kx).$$

With the substitution  $y = -x$ ,

$$\begin{aligned} \hat{\phi}(k) &= \frac{1}{2\pi} \int_{-\pi}^{\pi} \phi(x) e^{-ikx} \, dx \\ &= \frac{1}{2\pi} \int_{\pi}^{-\pi} \phi(-y) e^{iky} (-dy) \\ &= \frac{1}{2\pi} \int_{-\pi}^{\pi} \phi(-y) e^{iky} \, dy \\ &= \frac{1}{2\pi} \int_{-\pi}^{\pi} \phi(y) e^{-i(-k)y} \, dy \\ &= \hat{\phi}(-k). \end{aligned}$$

Therefore, using de Moivre's theorem,

$$\begin{aligned} S_n[\phi](x) &= \sum_{k=-n}^n \hat{\phi}(k) e^{ikx} \\ &= \hat{\phi}(0) + \sum_{k=1}^n \left( \hat{\phi}(k) e^{ikx} + \hat{\phi}(-k) e^{-ikx} \right) \\ &= \hat{\phi}(0) + \sum_{k=1}^n \hat{\phi}(k) (e^{ikx} + e^{-ikx}) \\ &= \hat{\phi}(0) + \sum_{k=1}^n \hat{\phi}(k) 2 \cos(kx) \\ &= \hat{\phi}(0) + 2 \sum_{k=1}^n \hat{\phi}(k) \cos(kx). \end{aligned}$$

□

### Question 3

*Wave equation with inhomogeneous boundary conditions:* Consider the boundary value problem:

$$\begin{cases} \partial_{tt}u(x, t) = \partial_{xx}u(x, t) & (x, t) \in (0, \pi) \times (0, \infty), \\ u(0, t) = -2 & t \in [0, \infty), \\ u(\pi, t) = 1 & t \in [0, \infty). \end{cases} \quad (2)$$

(i) Verify that

$$\bar{u}(x) = -2 + \frac{3}{\pi}x$$

is a stationary solution of the problem (i.e. one that does not depend on  $t$ ).

(ii) Assume now the initial conditions

$$\begin{aligned} u(x, 0) &= \Phi(x) = \frac{3}{\pi}x - 2 + 5 \sin(2x), \\ \partial_t u(x, 0) &= V(x) = \frac{1}{2} \sin(4x) + \frac{1}{3} \sin(11x). \end{aligned}$$

Let  $w(x, t)$  be the function such that  $u(x, t) = \bar{u}(x) + w(x, t)$ . State the initial boundary value problem satisfied by  $w$ .

(iii) Solve the initial boundary value problem for  $w$ , using the general form of the solution

$$w(x, t) = \sum_{j=0}^{\infty} \left( A_j \cos(jt) + B_j \sin(jt) \right) \sin(jx).$$

Then, state the solution  $u(x, t)$  of (2).

#### Q3 (i)

Since  $\bar{u}$  does not depend on  $t$ ,  $\partial_{tt}\bar{u} = \partial_t\bar{u} = 0$ . It is trivial to check that  $\bar{u}$  satisfies the initial boundary conditions  $\bar{u}(0) = -2$  and  $\bar{u}(\pi) = 1$ . Also

$$\partial_x \bar{u}(x) = \frac{3}{\pi}, \quad \partial_{xx} \bar{u}(x) = 0,$$

and so  $\partial_{tt}\bar{u} = \partial_{xx}\bar{u}$ . Therefore  $\bar{u}$  is a stationary solution to (2).

**Q3 (ii)**

$$\begin{cases} \partial_{tt}w(x, t) = \partial_{xx}w(x, t) & (x, t) \in (0, \pi) \times (0, \infty), \\ w(0, t) = 0 & t \in [0, \infty), \\ w(\pi, t) = 0 & t \in [0, \infty), \\ w(x, 0) = 5 \sin(2x) & x \in (0, \pi), \\ \partial_t w(x, 0) = \frac{1}{2} \sin(4x) + \frac{1}{3} \sin(11x) & x \in (0, \pi). \end{cases}$$

**Q3 (iii)**

Let

$$w(x, t) = \sum_{j=0}^{\infty} \left( A_j \cos(jt) + B_j \sin(jt) \right) \sin(jx).$$

This satisfies the conditions  $w(0, t) = 0$  and  $w(\pi, t) = 0$  because  $\sin 0 = \sin \pi = 0$ , so the  $\sin(jx)$  term annihilates the rest.

For the condition  $w(x, 0) = 5 \sin(2x)$ , we have

$$\begin{aligned} w(x, 0) &= \sum_{j=0}^{\infty} \left( A_j \cos(0) + B_j \sin(0) \right) \sin(jx) \\ &= \sum_{j=0}^{\infty} A_j \sin(jx) \\ &= 5 \sin(2x) \end{aligned}$$

which means that  $A_2 = 5$  and  $A_j = 0$  for all  $j \neq 2$ .

The derivatives are

$$\begin{aligned} \partial_t w(x, t) &= \sum_{j=0}^{\infty} \left( -j A_j \sin(jt) + j B_j \cos(jt) \right) \sin(jx) \\ \partial_{tt} w(x, t) &= \sum_{j=0}^{\infty} \left( -j^2 A_j \cos(jt) - j^2 B_j \sin(jt) \right) \sin(jx) \\ \partial_x w(x, t) &= \sum_{j=0}^{\infty} \left( A_j \cos(jt) + B_j \sin(jt) \right) j \cos(jx) \\ \partial_{xx} w(x, t) &= \sum_{j=0}^{\infty} \left( A_j \cos(jt) + B_j \sin(jt) \right) (-j^2) \sin(jx) \end{aligned}$$



So clearly  $\partial_{tt}w = \partial_{xx}w$ . Also to satisfy the final condition, we need

$$\begin{aligned}\partial_t w(x, 0) &= \sum_{j=0}^{\infty} \left( -jA_j \sin(0) + jB_j \cos(0) \right) \sin(jx) \\ &= \sum_{j=0}^{\infty} jB_j \sin(jx) \\ &= \frac{1}{2} \sin(4x) + \frac{1}{3} \sin(11x)\end{aligned}$$

which means that  $4B_4 = \frac{1}{2}$  so  $B_4 = \frac{1}{8}$ , and  $11B_{11} = \frac{1}{3}$  so  $B_{11} = \frac{1}{33}$ , and  $B_j = 0$  for all  $b \notin \{4, 11\}$ .

Therefore

$$w(x, t) = 5 \cos(2t) \sin(2x) + 2 \sin(4t) \sin(4x) + \frac{11}{3} \sin(11t) \sin(11x)$$

and therefore

$$u(x, t) = -2 + \frac{3}{\pi}x + 5 \cos(2t) \sin(2x) + 2 \sin(4t) \sin(4x) + \frac{11}{3} \sin(11t) \sin(11x).$$

## Question 4

*Fourier series:* Let  $a \in \mathbb{R} \setminus \mathbb{Z}$ . Compute the Fourier series of

$$\phi_a(x) = \frac{\pi}{\sin(\pi a)} e^{-iax}.$$

Then, assuming that

$$\lim_{n \rightarrow \infty} \int_{-\pi}^{\pi} |\phi_a(x) - S_n[\phi_a](x)|^2 dx = 0,$$

such that Parseval's identity holds, deduce that

$$\sum_{k \in \mathbb{Z}} \frac{1}{(k+a)^2} = \frac{\pi^2}{\sin^2(\pi a)}.$$

The coefficients are

$$\begin{aligned} \hat{\phi}_a(k) &= \frac{1}{2\pi} \int_{-\pi}^{\pi} \phi_a(x) e^{-ikx} dx \\ &= \frac{1}{2\pi} \int_{-\pi}^{\pi} \frac{\pi}{\sin(\pi a)} e^{-iax} e^{-ikx} dx \\ &= \frac{1}{2\sin(\pi a)} \int_{-\pi}^{\pi} e^{-i(a+k)x} dx \\ &= \frac{1}{2\sin(\pi a)} \left[ \frac{e^{-i(a+k)x}}{-i(a+k)} \right]_{-\pi}^{\pi} \\ &= \frac{i}{2\sin(\pi a)} \frac{e^{-i(a+k)\pi} - e^{i(a+k)\pi}}{(a+k)} \\ &= \frac{i(e^{-i(a+k)\pi} - e^{i(a+k)\pi})}{2(a+k)\sin(\pi a)} \\ &= \frac{i(-2i \sinh(i(a+k)\pi))}{2(a+k)\sin(\pi a)} \\ &= \frac{\sinh(i(a+k)\pi)}{(a+k)\sin(\pi a)} \\ &= \frac{\sin((a+k)\pi)}{(a+k)\sin(\pi a)}. \end{aligned}$$

Therefore

$$\begin{aligned} S_n[\phi_a](x) &= \sum_{k=-n}^n \hat{\phi}_a(k) e^{-ikx} \\ &= \sum_{k=-n}^n \frac{\sin((a+k)\pi)}{(a+k)\sin(\pi a)} e^{-ikx}. \end{aligned}$$

Parseval's identity says

$$\int_{-\pi}^{\pi} |\phi_a(x)|^2 dx = 2\pi \sum_{k \in \mathbb{Z}} |\hat{\phi}_a(k)|^2.$$

And so we get

$$\begin{aligned} \int_{-\pi}^{\pi} \left| \frac{\pi}{\sin(\pi a)} e^{-iax} \right|^2 dx &= 2\pi \sum_{k \in \mathbb{Z}} \left| \frac{\sin((a+k)\pi)}{(a+k)\sin(\pi a)} \right|^2 \\ \frac{\pi^2}{\sin^2(\pi a)} \int_{-\pi}^{\pi} |e^{-iax}|^2 dx &= 2\pi \frac{1}{\sin^2(\pi a)} \sum_{k \in \mathbb{Z}} \frac{\sin^2((a+k)\pi)}{(a+k)^2} \\ \frac{\pi^2}{\sin^2(\pi a)} \int_{-\pi}^{\pi} 1 dx &= \frac{2\pi}{\sin^2(\pi a)} \sum_{k \in \mathbb{Z}} \frac{(\sin(a\pi + k\pi))^2}{(a+k)^2} \\ \pi^2(2\pi) &= 2\pi \sum_{k \in \mathbb{Z}} \frac{(\sin(a\pi) \cos(k\pi) + \cos(a\pi) \sin(k\pi))^2}{(a+k)^2} \\ \pi^2 &= \sum_{k \in \mathbb{Z}} \frac{\sin^2(a\pi) \cos^2(k\pi)}{(a+k)^2} \\ \pi^2 &= \sum_{k \in \mathbb{Z}} \frac{\sin^2(a\pi)}{(a+k)^2} \\ \frac{\pi^2}{\sin^2(a\pi)} &= \sum_{k \in \mathbb{Z}} \frac{1}{(a+k)^2} \end{aligned}$$

□